pulse/lib/pulse/core/PulseCore.MemoryAlt.fst
@@ -27,48 +27,9 @@ module MSTTotal = PulseCore.MonotonicStateMonad
 module S = FStar.Set
 module Frac = PulseCore.FractionalPermission
 module L = FStar.List.Tot
-
-
-let raw_inv_store : Type u#(a + 3) = erased (H0.heap u#(a + 2))
-
-(** [sel] is a ghost read of the value contained in a heap reference *)
-noeq
-type cell : Type u#(a + 1) =
-  | Ref : a:Type u#a ->
-          p:pcm a ->
-          frac:Frac.perm{ frac `Frac.lesser_equal_perm` Frac.full_perm } ->
-          v:a { frac == Frac.full_perm ==> p.refine v } ->
-          cell
-
-assume
-val sel (i:nat) (m:H0.heap u#a) : option (cell u#a)
-
-assume
-val sel_empty (i:nat)
-  : Lemma 
-    (ensures sel i H0.empty_heap == None)
-    [SMTPat (sel i H0.empty_heap)
-    ]
-
 module PA = PulseCore.PCM.Agreement
 
-let inv_store_has_only_invs (l:raw_inv_store u#a) : prop =
-  forall i.
-    match sel i l with
-    | None -> True
-    | Some cell ->
-      let Ref a p f v = cell in
-      a == PA.agreement H2.slprop /\
-      p == PA.pcm_agreement #H2.slprop
-  
-let istore = raw_inv_store
-
-// let join_istore (h0 h1:istore)
-//   : Lemma 
-//     (requires H0.disjoint h0 h1)
-//     (ensures (inv_store_has_only_invs (H0.join h0 h1)))
-//     [SMTPat ((inv_store_has_only_invs (H0.join h0 h1)))]
-//   = admit()
+let istore : Type u#(a + 3) = erased (H0.heap u#(a + 2))
 
 noeq
 type iheap : Type u#(a + 3) = {
@@ -428,13 +389,13 @@ module W = FStar.Witnessed.Core
 let sl_pure_imp (p:prop) (q: squash p -> slprop) : slprop =
   as_slprop (fun (h:iheap) -> p ==> q () h)
 
-let cell_pred_pre (c:cell) =
-  let Ref a pcm _ _ = c in
+let cell_pred_pre (c:H0.cell) =
+  let H0.Ref a pcm _ _ = c in
   a == PA.agreement H2.slprop /\
   pcm == PA.pcm_agreement #H2.slprop
 
-let cell_pred_post (c:cell) (_:squash (cell_pred_pre c)) =
-  let Ref _ _ _ v = c in
+let cell_pred_post (c:H0.cell) (_:squash (cell_pred_pre c)) =
+  let H0.Ref _ _ _ v = c in
   let v : PA.agreement H2.slprop = v in
   match v with
   | None -> emp
@@ -443,7 +404,7 @@ let cell_pred_post (c:cell) (_:squash (cell_pred_pre c)) =
 
 let invariant_of_one_cell (addr:nat) (e:inames) (l:istore u#a) : slprop u#a =
   if addr `S.mem` e then emp
-  else match sel addr l with
+  else match H0.select addr l with
        | Some c -> 
          sl_pure_imp 
           (cell_pred_pre c)
@@ -460,10 +421,10 @@ let rec istore_invariant
 
 let istore_evolves : FStar.Preorder.preorder istore =
   fun (l1 l2 : istore) ->
-    forall addr. Some? (sel addr l1) ==> sel addr l1 == sel addr l2
+    forall addr. Some? (H0.select addr l1) ==> H0.select addr l1 == H0.select addr l2
 
 let inames_in (e:inames) (l:istore) : prop = 
-  forall i. Set.mem i e ==> Some? (sel i l)
+  forall i. Set.mem i e ==> Some? (H0.select i l)
 
 let heap_ctr_valid (ctr:nat) (ghost_ctr:nat) (iname_ctr:nat) (h:iheap u#a) : prop =
     h.concrete `H2.free_above_addr CONCRETE` ctr /\
@@ -507,10 +468,10 @@ let frame_related_mems (fp0 fp1:slprop u#a) e (m0:hmem_with_inv_except e fp0) (m
       mem_evolves m0 m1
 
 let iname_for_p (i:iname) (p:slprop) (m:istore) =
-  match sel i m with
+  match H0.select i m with
   | None -> False
   | Some cell ->
-    let Ref a pcm _ v = cell in
+    let H0.Ref a pcm _ v = cell in
     a == PA.agreement H2.slprop /\
     pcm == PA.pcm_agreement #H2.slprop /\ (
     let v : PA.agreement H2.slprop = cell.v in
@@ -602,7 +563,7 @@ let rec move_invariant (e:inames) (l:istore) (p:slprop) (from:nat)
   };
   if i = from
   then (
-    let Some c = sel i l in
+    let Some c = H0.select i l in
     assert (cell_pred_pre c);
     sl_pure_imp_elim (cell_pred_pre c) (cell_pred_post c);
     assert (invariant_of_one_cell from e l == p);
@@ -836,12 +797,12 @@ let sl_pure_imp_big (p:prop) (q: squash p -> slprop)
 let invariant_of_one_cell_is_big (from:nat) (e:inames) (i:istore)
 : Lemma (is_big (invariant_of_one_cell from e i))
 = if from `S.mem` e then ()
-  else match sel from i with
+  else match H0.select from i with
        | None -> ()
        | Some c ->
          introduce cell_pred_pre c ==> is_big (cell_pred_post c ())
          with _ . (
-            let Ref _ _ _ v = c in
+            let H0.Ref _ _ _ v = c in
             let v : PA.agreement H2.slprop = v in
             match v with
             | None -> ()
@@ -904,7 +865,7 @@ let new_invariant_pre_action (e:inames) (p:slprop { is_big p })
         Ghost.hide <| H0.extend #_ #(PA.pcm_agreement) (Some (down p)) iname m0.iheap.invariants
     in
     let x : iname_ref = dfst res in
-    let inv1 : raw_inv_store (* erased (H0.full_hheap (H0.pts_to x (Some (down p)))) *) = dsnd res in
+    let inv1 : istore (* erased (H0.full_hheap (H0.pts_to x (Some (down p)))) *) = dsnd res in
     (* Need a lemma about extend from H0 *)
     // assume (forall i. i < iname ==> sel i m0.iheap.invariants == sel i inv1);
     // assume (sel iname inv1 == Some (Ref _ (PA.pcm_agreement #H2.slprop) Frac.full_perm (Some (down p))));
@@ -1025,790 +986,790 @@ let new_invariant' (e:inames) (p:slprop { is_big p })
 : pst_ghost_action_except iname_ref e p (fun i -> iname_ref_pts_to i p)
 = lift_tot_action (refined_pre_action_as_action (new_invariant_pre_action e p))
 
-let new_invariant_tot_action (e:inames) (p:slprop) (m0:hmem_with_inv_except e p{ e `inames_in` m0.locks })
-  : Pure (iname & hmem_with_inv_except e emp)
-         (requires True)
-         (ensures fun (i, m1) ->
-           iname_for_p_mem i p m1 /\
-           frame_related_mems p emp e m0 m1 /\
-           mem_evolves m0 m1)
-  = let (| i, l1 |) = extend_lock_store e m0.locks p in
-    let m1 = { m0 with locks = l1 } in
-    assert (lock_store_invariant e m1.locks ==
-            p `star` lock_store_invariant e m0.locks);
-    calc (equiv) {
-      linv e m1;
-        (equiv) {}
-      (lock_store_invariant e m1.locks
-        `star`
-       ctr_validity m1.ctr m1.ghost_ctr (heap_of_mem m1));
-        (equiv) {}
-      ((p `star` lock_store_invariant e m0.locks)
-        `star`
-       ctr_validity m1.ctr m1.ghost_ctr (heap_of_mem m1));
-        (equiv) {
-          H.star_associative p (lock_store_invariant e m0.locks) (ctr_validity m1.ctr m1.ghost_ctr (heap_of_mem m1))
-         }
-      (p `star` (lock_store_invariant e m0.locks
-        `star`
-       ctr_validity m1.ctr m1.ghost_ctr (heap_of_mem m1)));
-        (equiv) { }
-      (p `star` linv e m0);
-    };
-    assert (iname_for_p_mem i p m1);
-    assert (lock_store_evolves m0.locks l1);
-    assert (mem_evolves m0 m1);
-    hmem_with_inv_equiv e m0 p;
-    assert (interp (p `star` lock_store_invariant e m0.locks) m1);
-    assert (interp (lock_store_invariant e m1.locks) m1);
-    H.emp_unit (lock_store_invariant e m1.locks);
-    H.star_commutative (lock_store_invariant e m1.locks) emp;
-    assert (interp (emp `star` lock_store_invariant e m1.locks) m1);
-    hmem_with_inv_equiv e m1 emp;
-    let m1 : hmem_with_inv_except e emp = m1 in
-    let aux (frame:slprop)
-      : Lemma
-        (requires interp ((p `star` frame) `star` linv e m0) m0)
-        (ensures interp ((emp `star` frame) `star` linv e m1) m1 /\
-                 mem_evolves m0 m1 /\
-                 (forall (mp:mprop frame). mp (core_mem m0) <==> mp (core_mem m1)))
-        [SMTPat (p `star` frame)]
-      = assert (interp ((p `star` frame) `star` linv e m0) m1);
-        calc (equiv) {
-          ((p `star` frame) `star` linv e m0);
-            (equiv) {
-                      H.star_commutative p frame;
-                      H.star_congruence (p `star` frame) (linv e m0) (frame `star` p) (linv e m0);
-                      H.star_associative frame p (linv e m0)
-                    }
-          (frame `star` (p `star` linv e m0));
-            (equiv) {
-                      H.star_congruence frame (p `star` linv e m0) frame (linv e m1)
-                    }
-          (frame `star` linv e m1);
-            (equiv) {
-                       H.emp_unit (frame `star` linv e m1);
-                       H.star_commutative (frame `star` linv e m1) emp;
-                       H.star_associative emp frame (linv e m1)
-                    }
-          ((emp `star` frame) `star` linv e m1);
-        };
-        assert (interp ((emp `star` frame) `star` linv e m1) m1)
-    in
-    assert (frame_related_mems p emp e m0 m1);
-    ( i, m1 )
+// let new_invariant_tot_action (e:inames) (p:slprop) (m0:hmem_with_inv_except e p{ e `inames_in` m0.locks })
+//   : Pure (iname & hmem_with_inv_except e emp)
+//          (requires True)
+//          (ensures fun (i, m1) ->
+//            iname_for_p_mem i p m1 /\
+//            frame_related_mems p emp e m0 m1 /\
+//            mem_evolves m0 m1)
+//   = let (| i, l1 |) = extend_lock_store e m0.locks p in
+//     let m1 = { m0 with locks = l1 } in
+//     assert (lock_store_invariant e m1.locks ==
+//             p `star` lock_store_invariant e m0.locks);
+//     calc (equiv) {
+//       linv e m1;
+//         (equiv) {}
+//       (lock_store_invariant e m1.locks
+//         `star`
+//        ctr_validity m1.ctr m1.ghost_ctr (heap_of_mem m1));
+//         (equiv) {}
+//       ((p `star` lock_store_invariant e m0.locks)
+//         `star`
+//        ctr_validity m1.ctr m1.ghost_ctr (heap_of_mem m1));
+//         (equiv) {
+//           H.star_associative p (lock_store_invariant e m0.locks) (ctr_validity m1.ctr m1.ghost_ctr (heap_of_mem m1))
+//          }
+//       (p `star` (lock_store_invariant e m0.locks
+//         `star`
+//        ctr_validity m1.ctr m1.ghost_ctr (heap_of_mem m1)));
+//         (equiv) { }
+//       (p `star` linv e m0);
+//     };
+//     assert (iname_for_p_mem i p m1);
+//     assert (lock_store_evolves m0.locks l1);
+//     assert (mem_evolves m0 m1);
+//     hmem_with_inv_equiv e m0 p;
+//     assert (interp (p `star` lock_store_invariant e m0.locks) m1);
+//     assert (interp (lock_store_invariant e m1.locks) m1);
+//     H.emp_unit (lock_store_invariant e m1.locks);
+//     H.star_commutative (lock_store_invariant e m1.locks) emp;
+//     assert (interp (emp `star` lock_store_invariant e m1.locks) m1);
+//     hmem_with_inv_equiv e m1 emp;
+//     let m1 : hmem_with_inv_except e emp = m1 in
+//     let aux (frame:slprop)
+//       : Lemma
+//         (requires interp ((p `star` frame) `star` linv e m0) m0)
+//         (ensures interp ((emp `star` frame) `star` linv e m1) m1 /\
+//                  mem_evolves m0 m1 /\
+//                  (forall (mp:mprop frame). mp (core_mem m0) <==> mp (core_mem m1)))
+//         [SMTPat (p `star` frame)]
+//       = assert (interp ((p `star` frame) `star` linv e m0) m1);
+//         calc (equiv) {
+//           ((p `star` frame) `star` linv e m0);
+//             (equiv) {
+//                       H.star_commutative p frame;
+//                       H.star_congruence (p `star` frame) (linv e m0) (frame `star` p) (linv e m0);
+//                       H.star_associative frame p (linv e m0)
+//                     }
+//           (frame `star` (p `star` linv e m0));
+//             (equiv) {
+//                       H.star_congruence frame (p `star` linv e m0) frame (linv e m1)
+//                     }
+//           (frame `star` linv e m1);
+//             (equiv) {
+//                        H.emp_unit (frame `star` linv e m1);
+//                        H.star_commutative (frame `star` linv e m1) emp;
+//                        H.star_associative emp frame (linv e m1)
+//                     }
+//           ((emp `star` frame) `star` linv e m1);
+//         };
+//         assert (interp ((emp `star` frame) `star` linv e m1) m1)
+//     in
+//     assert (frame_related_mems p emp e m0 m1);
+//     ( i, m1 )
 
-let name_is_ok (i:iname) (m0:full_mem u#a) : prop = i < List.Tot.length m0.locks
+// let name_is_ok (i:iname) (m0:full_mem u#a) : prop = i < List.Tot.length m0.locks
 
-let witnessed_name_is_ok (i:iname) = W.witnessed (full_mem u#a) mem_evolves (name_is_ok i)
+// let witnessed_name_is_ok (i:iname) = W.witnessed (full_mem u#a) mem_evolves (name_is_ok i)
 
 
 
-let pre_inv_aux (p:slprop u#a) : Type0 = i:erased iname & witnessed_name_is_ok u#a i
-let inv (p:slprop u#a) = i:erased iname & witnessed_name_is_ok u#a i & (i >--> p)
+// let pre_inv_aux (p:slprop u#a) : Type0 = i:erased iname & witnessed_name_is_ok u#a i
+// let inv (p:slprop u#a) = i:erased iname & witnessed_name_is_ok u#a i & (i >--> p)
 
-let pre_inv_of_inv (#p:slprop u#a) (i:inv p) : pre_inv u#a = let (|i, w, _|) = i in (|i,w|)
-let name_of_pre_inv (i:pre_inv) = dfst i
+// let pre_inv_of_inv (#p:slprop u#a) (i:inv p) : pre_inv u#a = let (|i, w, _|) = i in (|i,w|)
+// let name_of_pre_inv (i:pre_inv) = dfst i
 
-let rec recall_all (ctx:list (pre_inv u#a))
-  : MSTTotal.mst #(full_mem u#a) mem_evolves unit 
-    (requires fun _ -> True)
-    (ensures fun m0 _ m1 -> m0==m1 /\ (forall (i:pre_inv u#a). i `List.Tot.memP` ctx ==> name_is_ok (name_of_pre_inv i) m0))
-  = match ctx with
-    | [] -> MST.weaken <| MST.return ()
-    | hd::tl ->
-      let (| q, i |) = hd in
-      let i : W.witnessed (full_mem u#a) mem_evolves (name_is_ok q) = i in
-      MST.weaken <|
-      MST.bind (MST.recall (name_is_ok q) i) (fun _ -> recall_all u#a tl)
+// let rec recall_all (ctx:list (pre_inv u#a))
+//   : MSTTotal.mst #(full_mem u#a) mem_evolves unit 
+//     (requires fun _ -> True)
+//     (ensures fun m0 _ m1 -> m0==m1 /\ (forall (i:pre_inv u#a). i `List.Tot.memP` ctx ==> name_is_ok (name_of_pre_inv i) m0))
+//   = match ctx with
+//     | [] -> MST.weaken <| MST.return ()
+//     | hd::tl ->
+//       let (| q, i |) = hd in
+//       let i : W.witnessed (full_mem u#a) mem_evolves (name_is_ok q) = i in
+//       MST.weaken <|
+//       MST.bind (MST.recall (name_is_ok q) i) (fun _ -> recall_all u#a tl)
 
-let distinct_invariants_have_distinct_names
-      (e:inames)
-      (p:slprop u#a)
-      (q:slprop u#a { p =!= q })
-      (i:inv p)
-      (j:inv q)
-      (frame:slprop u#a)
-: _MstTot (squash (name_of_inv i =!= name_of_inv j)) e (emp u#a) (fun _ -> emp u#a) frame
-= let (| ni, wi, toki |) = i in
-  let (| nj, wj, tokj |) = j in
-  let toki : (ni >--> p) = toki in
-  let tokj : (nj >--> q) = tokj in
-  let elim 
-    : _mst_tot_aux
-        (squash (name_of_inv i =!= name_of_inv j))
-        e
-        emp
-        (fun _ -> emp)
-        frame
-        (fun _ -> name_of_inv i =!= name_of_inv j)
-    = fun m0 -> MST.weaken <| MST.return ()
-  in
-  MST.weaken <|
-  MST.bind (MST.recall _ toki) (fun _ ->
-  MST.bind (MST.recall _ tokj) (fun _ ->
-            with_get_aux elim))
+// let distinct_invariants_have_distinct_names
+//       (e:inames)
+//       (p:slprop u#a)
+//       (q:slprop u#a { p =!= q })
+//       (i:inv p)
+//       (j:inv q)
+//       (frame:slprop u#a)
+// : _MstTot (squash (name_of_inv i =!= name_of_inv j)) e (emp u#a) (fun _ -> emp u#a) frame
+// = let (| ni, wi, toki |) = i in
+//   let (| nj, wj, tokj |) = j in
+//   let toki : (ni >--> p) = toki in
+//   let tokj : (nj >--> q) = tokj in
+//   let elim 
+//     : _mst_tot_aux
+//         (squash (name_of_inv i =!= name_of_inv j))
+//         e
+//         emp
+//         (fun _ -> emp)
+//         frame
+//         (fun _ -> name_of_inv i =!= name_of_inv j)
+//     = fun m0 -> MST.weaken <| MST.return ()
+//   in
+//   MST.weaken <|
+//   MST.bind (MST.recall _ toki) (fun _ ->
+//   MST.bind (MST.recall _ tokj) (fun _ ->
+//             with_get_aux elim))
 
-let invariant_name_identifies_invariant
-      (e:inames)
-      (p:slprop)
-      (q:slprop)
-      (i:inv p)
-      (j:inv q { name_of_inv i == name_of_inv j })
-      (frame:slprop)
-: _MstTot (squash (p == q /\ i == j)) e emp (fun _ -> emp) frame
-= let (| ni, wi, toki |) = i in
-  let (| nj, wj, tokj |) = j in
-  assert (ni == nj);
-  let elim 
-    : _mst_tot_aux
-        (squash (p == q /\ i == j))
-        e
-        emp
-        (fun _ -> emp)
-        frame
-        (fun m -> iname_for_p_mem ni p m /\ iname_for_p_mem nj q m)
-    = fun _ -> 
-        W.witnessed_proof_irrelevant _ _ _ wi wj;
-        W.witnessed_proof_irrelevant _ _ _ toki tokj;
-        MST.weaken <| MST.return ()
-  in
-  MST.weaken <|
-  MST.bind (MST.recall _ toki) (fun _ ->
-  MST.bind (MST.recall _ tokj) (fun _ ->
-            with_get_aux elim))
+// let invariant_name_identifies_invariant
+//       (e:inames)
+//       (p:slprop)
+//       (q:slprop)
+//       (i:inv p)
+//       (j:inv q { name_of_inv i == name_of_inv j })
+//       (frame:slprop)
+// : _MstTot (squash (p == q /\ i == j)) e emp (fun _ -> emp) frame
+// = let (| ni, wi, toki |) = i in
+//   let (| nj, wj, tokj |) = j in
+//   assert (ni == nj);
+//   let elim 
+//     : _mst_tot_aux
+//         (squash (p == q /\ i == j))
+//         e
+//         emp
+//         (fun _ -> emp)
+//         frame
+//         (fun m -> iname_for_p_mem ni p m /\ iname_for_p_mem nj q m)
+//     = fun _ -> 
+//         W.witnessed_proof_irrelevant _ _ _ wi wj;
+//         W.witnessed_proof_irrelevant _ _ _ toki tokj;
+//         MST.weaken <| MST.return ()
+//   in
+//   MST.weaken <|
+//   MST.bind (MST.recall _ toki) (fun _ ->
+//   MST.bind (MST.recall _ tokj) (fun _ ->
+//             with_get_aux elim))
   
-let fresh_invariant (e:inames) (p:slprop u#a) (ctx:list (pre_inv u#a)) (frame:slprop u#a)
-  : _MstTot (i:inv p { fresh_wrt ctx (name_of_inv i)}) e p (fun _ -> emp u#a) frame
-  = let elim
-    : _mst_tot_aux
-        (i:inv p { fresh_wrt ctx (name_of_inv i)})
-        e
-        p
-        (fun _ -> emp)
-        frame
-        (fun m0 -> 
-          (forall i. i `List.Tot.memP` ctx ==> name_is_ok (name_of_pre_inv i) m0))
-    = fun m0 ->
-        ac_reasoning_for_m_frame_preserving p frame (locks_invariant e m0) m0;
-        assert (interp (p `star` locks_invariant e m0) m0);
-        let r = new_invariant_tot_action e p m0 in
-        let ( i, m1 ) = r in
-        assert (i == List.Tot.length m0.locks);
-        assert (not (Set.mem i e));
-        assert (mem_evolves m0 m1);
-        iname_for_p_stable i p;
-        MST.weaken <|
-        MST.bind (MSTTotal.put #full_mem #mem_evolves m1) (fun _ ->
-        MST.bind (MST.witness #full_mem #mem_evolves (iname_for_p_mem i p)) (fun w ->
-        MST.bind (MST.witness #full_mem #mem_evolves (name_is_ok i)) (fun w0 ->
-        let i : inv p = (| hide i, w0, w |) in
-        assert (fresh_wrt ctx (name_of_inv i));
-        MST.weaken #_ #_ #(i:inv p {fresh_wrt ctx (name_of_inv i)})
-          #_ #_
-          #(fun m0 -> True)
-          #(fun m0 _ m1 -> m0==m1)
-          <| MST.return i)))
-    in
-    MST.weaken <|
-    MST.bind (recall_all ctx) (fun _ -> with_get_aux elim)
+// let fresh_invariant (e:inames) (p:slprop u#a) (ctx:list (pre_inv u#a)) (frame:slprop u#a)
+//   : _MstTot (i:inv p { fresh_wrt ctx (name_of_inv i)}) e p (fun _ -> emp u#a) frame
+//   = let elim
+//     : _mst_tot_aux
+//         (i:inv p { fresh_wrt ctx (name_of_inv i)})
+//         e
+//         p
+//         (fun _ -> emp)
+//         frame
+//         (fun m0 -> 
+//           (forall i. i `List.Tot.memP` ctx ==> name_is_ok (name_of_pre_inv i) m0))
+//     = fun m0 ->
+//         ac_reasoning_for_m_frame_preserving p frame (locks_invariant e m0) m0;
+//         assert (interp (p `star` locks_invariant e m0) m0);
+//         let r = new_invariant_tot_action e p m0 in
+//         let ( i, m1 ) = r in
+//         assert (i == List.Tot.length m0.locks);
+//         assert (not (Set.mem i e));
+//         assert (mem_evolves m0 m1);
+//         iname_for_p_stable i p;
+//         MST.weaken <|
+//         MST.bind (MSTTotal.put #full_mem #mem_evolves m1) (fun _ ->
+//         MST.bind (MST.witness #full_mem #mem_evolves (iname_for_p_mem i p)) (fun w ->
+//         MST.bind (MST.witness #full_mem #mem_evolves (name_is_ok i)) (fun w0 ->
+//         let i : inv p = (| hide i, w0, w |) in
+//         assert (fresh_wrt ctx (name_of_inv i));
+//         MST.weaken #_ #_ #(i:inv p {fresh_wrt ctx (name_of_inv i)})
+//           #_ #_
+//           #(fun m0 -> True)
+//           #(fun m0 _ m1 -> m0==m1)
+//           <| MST.return i)))
+//     in
+//     MST.weaken <|
+//     MST.bind (recall_all ctx) (fun _ -> with_get_aux elim)
 
-let new_invariant (e:inames) (p:slprop) (frame:slprop)
-  : _MstTot (inv p) e p (fun _ -> emp) frame
-  = fresh_invariant e p [] frame
+// let new_invariant (e:inames) (p:slprop) (frame:slprop)
+//   : _MstTot (inv p) e p (fun _ -> emp) frame
+//   = fresh_invariant e p [] frame
 
-let rearrange_invariant (p q r : slprop) (q0 q1:slprop)
-  : Lemma
-    (requires q `equiv` (q0 `star` q1))
-    (ensures  (p `star` (q `star` r)) `equiv`
-              ((q0 `star` p) `star` (q1 `star` r)))
-  = calc (equiv)
-    {
-       p `star` (q `star` r);
-         (equiv)
-           {
-             calc (equiv)
-             {
-               (q `star` r);
-                 (equiv) {
-                             star_congruence q r (q0 `star` q1) r
-                         }
-               (q0 `star` q1) `star` r;
-             };
-             star_congruence p (q `star` r) p ((q0 `star` q1) `star` r)
-           }
-       (p `star` ((q0 `star` q1) `star` r));
-          (equiv) {
-                    star_associative q0 q1 r;
-                    star_congruence p ((q0 `star` q1) `star` r)
-                                    p (q0 `star` (q1 `star` r));
-                    star_associative p q0 (q1 `star` r)
-                  }
-       (p `star` q0) `star` (q1 `star` r);
-          (equiv) {
-                     star_commutative p q0;
-                     star_congruence (p `star` q0) (q1 `star` r)
-                                     (q0 `star` p)  (q1 `star` r)
-                  }
-       (q0 `star` p) `star` (q1 `star` r);
-    }
+// let rearrange_invariant (p q r : slprop) (q0 q1:slprop)
+//   : Lemma
+//     (requires q `equiv` (q0 `star` q1))
+//     (ensures  (p `star` (q `star` r)) `equiv`
+//               ((q0 `star` p) `star` (q1 `star` r)))
+//   = calc (equiv)
+//     {
+//        p `star` (q `star` r);
+//          (equiv)
+//            {
+//              calc (equiv)
+//              {
+//                (q `star` r);
+//                  (equiv) {
+//                              star_congruence q r (q0 `star` q1) r
+//                          }
+//                (q0 `star` q1) `star` r;
+//              };
+//              star_congruence p (q `star` r) p ((q0 `star` q1) `star` r)
+//            }
+//        (p `star` ((q0 `star` q1) `star` r));
+//           (equiv) {
+//                     star_associative q0 q1 r;
+//                     star_congruence p ((q0 `star` q1) `star` r)
+//                                     p (q0 `star` (q1 `star` r));
+//                     star_associative p q0 (q1 `star` r)
+//                   }
+//        (p `star` q0) `star` (q1 `star` r);
+//           (equiv) {
+//                      star_commutative p q0;
+//                      star_congruence (p `star` q0) (q1 `star` r)
+//                                      (q0 `star` p)  (q1 `star` r)
+//                   }
+//        (q0 `star` p) `star` (q1 `star` r);
+//     }
 
-let preserves_frame_invariant (fp fp':slprop)
-                              (opened_invariants:inames)
-                              (p:slprop)
-                              (i:inv p{not (mem_inv opened_invariants i)})
-                              (m0:hmem_with_inv_except (add_inv opened_invariants i) (p `star` fp))
-                              (m1:mem)
-    : Lemma
-      (requires preserves_frame (set_add (name_of_inv i) opened_invariants) (p `star` fp) (p `star` fp') m0 m1 /\
-                interp (fp' `star` linv opened_invariants m1) m1 /\
-                inames_ok opened_invariants m1 /\
-                (lock_store_invariant opened_invariants m0.locks `equiv`
-                   (p `star` lock_store_invariant (set_add (name_of_inv i) opened_invariants) m0.locks)) /\
-                (lock_store_invariant opened_invariants m1.locks `equiv`
-                 (p `star` lock_store_invariant (set_add (name_of_inv i) opened_invariants) m1.locks)))
-      (ensures  preserves_frame opened_invariants fp fp' m0 m1)
-    =
-      let aux (frame:slprop)
-        : Lemma
-           (requires
-             interp ((fp `star` frame) `star` linv opened_invariants m0) m0)
-           (ensures
-             interp ((fp' `star` frame) `star` linv opened_invariants m1) m1 /\
-             (forall (f_frame:mprop frame). f_frame (core_mem m0) == f_frame (core_mem m1)))
-           [SMTPat()]
-        = rearrange_invariant (fp `star` frame) (lock_store_invariant opened_invariants m0.locks) (ctr_validity m0.ctr m0.ghost_ctr (heap_of_mem m0))
-                                                p (lock_store_invariant (set_add (name_of_inv i) opened_invariants) m0.locks);
-          assert (interp ((p `star` (fp `star` frame)) `star` linv (set_add (name_of_inv i) opened_invariants) m0) m0);
-          star_associative p fp frame;
-          star_congruence (p `star` (fp `star` frame)) (linv (set_add (name_of_inv i) opened_invariants) m0)
-                          ((p `star` fp) `star` frame)  (linv (set_add (name_of_inv i) opened_invariants) m0);
-          assert (interp (((p `star` fp) `star` frame) `star` linv (set_add (name_of_inv i) opened_invariants) m0) m0);
-          assert (interp (((p `star` fp') `star` frame) `star` linv (set_add (name_of_inv i) opened_invariants) m1) m1);
-          star_associative p fp' frame;
-          star_congruence ((p `star` fp') `star` frame) (linv (set_add (name_of_inv i) opened_invariants) m1)
-                          (p `star` (fp' `star` frame)) (linv (set_add (name_of_inv i) opened_invariants) m1);
-          assert (interp ((p `star` (fp' `star` frame)) `star` linv (set_add (name_of_inv i) opened_invariants) m1) m1);
-          rearrange_invariant (fp' `star` frame) (lock_store_invariant opened_invariants m1.locks) (ctr_validity m1.ctr m1.ghost_ctr (heap_of_mem m1))
-                                                 p (lock_store_invariant (set_add (name_of_inv i) opened_invariants) m1.locks);
-          assert (interp ((fp' `star` frame) `star` linv opened_invariants m1) m1);
-          ()
-      in
-      ()
+// let preserves_frame_invariant (fp fp':slprop)
+//                               (opened_invariants:inames)
+//                               (p:slprop)
+//                               (i:inv p{not (mem_inv opened_invariants i)})
+//                               (m0:hmem_with_inv_except (add_inv opened_invariants i) (p `star` fp))
+//                               (m1:mem)
+//     : Lemma
+//       (requires preserves_frame (set_add (name_of_inv i) opened_invariants) (p `star` fp) (p `star` fp') m0 m1 /\
+//                 interp (fp' `star` linv opened_invariants m1) m1 /\
+//                 inames_ok opened_invariants m1 /\
+//                 (lock_store_invariant opened_invariants m0.locks `equiv`
+//                    (p `star` lock_store_invariant (set_add (name_of_inv i) opened_invariants) m0.locks)) /\
+//                 (lock_store_invariant opened_invariants m1.locks `equiv`
+//                  (p `star` lock_store_invariant (set_add (name_of_inv i) opened_invariants) m1.locks)))
+//       (ensures  preserves_frame opened_invariants fp fp' m0 m1)
+//     =
+//       let aux (frame:slprop)
+//         : Lemma
+//            (requires
+//              interp ((fp `star` frame) `star` linv opened_invariants m0) m0)
+//            (ensures
+//              interp ((fp' `star` frame) `star` linv opened_invariants m1) m1 /\
+//              (forall (f_frame:mprop frame). f_frame (core_mem m0) == f_frame (core_mem m1)))
+//            [SMTPat()]
+//         = rearrange_invariant (fp `star` frame) (lock_store_invariant opened_invariants m0.locks) (ctr_validity m0.ctr m0.ghost_ctr (heap_of_mem m0))
+//                                                 p (lock_store_invariant (set_add (name_of_inv i) opened_invariants) m0.locks);
+//           assert (interp ((p `star` (fp `star` frame)) `star` linv (set_add (name_of_inv i) opened_invariants) m0) m0);
+//           star_associative p fp frame;
+//           star_congruence (p `star` (fp `star` frame)) (linv (set_add (name_of_inv i) opened_invariants) m0)
+//                           ((p `star` fp) `star` frame)  (linv (set_add (name_of_inv i) opened_invariants) m0);
+//           assert (interp (((p `star` fp) `star` frame) `star` linv (set_add (name_of_inv i) opened_invariants) m0) m0);
+//           assert (interp (((p `star` fp') `star` frame) `star` linv (set_add (name_of_inv i) opened_invariants) m1) m1);
+//           star_associative p fp' frame;
+//           star_congruence ((p `star` fp') `star` frame) (linv (set_add (name_of_inv i) opened_invariants) m1)
+//                           (p `star` (fp' `star` frame)) (linv (set_add (name_of_inv i) opened_invariants) m1);
+//           assert (interp ((p `star` (fp' `star` frame)) `star` linv (set_add (name_of_inv i) opened_invariants) m1) m1);
+//           rearrange_invariant (fp' `star` frame) (lock_store_invariant opened_invariants m1.locks) (ctr_validity m1.ctr m1.ghost_ctr (heap_of_mem m1))
+//                                                  p (lock_store_invariant (set_add (name_of_inv i) opened_invariants) m1.locks);
+//           assert (interp ((fp' `star` frame) `star` linv opened_invariants m1) m1);
+//           ()
+//       in
+//       ()
 
 
-let equiv_ext_right (p q r:slprop)
-  : Lemma
-      (requires q `equiv` r)
-      (ensures (p `star` q) `equiv` (p `star` r))
-  = calc (equiv) {
-      p `star` q;
-         (equiv) { star_commutative p q }
-      q `star` p;
-         (equiv) { slprop_extensionality q r }
-      r `star` p;
-         (equiv) { star_commutative p r }
-      p `star` r;
-    }
+// let equiv_ext_right (p q r:slprop)
+//   : Lemma
+//       (requires q `equiv` r)
+//       (ensures (p `star` q) `equiv` (p `star` r))
+//   = calc (equiv) {
+//       p `star` q;
+//          (equiv) { star_commutative p q }
+//       q `star` p;
+//          (equiv) { slprop_extensionality q r }
+//       r `star` p;
+//          (equiv) { star_commutative p r }
+//       p `star` r;
+//     }
 
-let with_inv_helper (fp frame ls1 ctr p ls2:slprop)
-  : Lemma
-      (requires ls1 `equiv` (p `star` ls2))
-      (ensures
-        (fp `star` frame `star` (ls1 `star` ctr)) `equiv`
-        (p `star` fp `star` frame `star` (ls2 `star` ctr)))
-  = calc (equiv) {
-      ls1 `star` ctr;
-         (equiv) { slprop_extensionality ls1 (p `star` ls2) }
-      p `star` ls2 `star` ctr;
-    };
-    calc (equiv) {
-      p `star` ls2 `star` ctr;
-         (equiv) { star_associative p ls2 ctr }
-      p `star` (ls2 `star` ctr);
-    };
-    calc (equiv) {
-      fp `star` frame `star` p;
-         (equiv) { star_commutative (fp `star` frame) p }
-      p `star` (fp `star` frame);
-         (equiv) { star_associative p fp frame }
-      p `star` fp `star` frame;
-    };
-    calc (equiv) {
-      fp `star` frame `star` (ls1 `star` ctr);
-         (equiv) { equiv_ext_right (fp `star` frame)
-                     (ls1 `star` ctr)
-                     (p `star` ls2 `star` ctr) }
-      (fp `star` frame) `star` (p `star` ls2 `star` ctr);
-         (equiv) { equiv_ext_right (fp `star` frame)
-                     (p `star` ls2 `star` ctr)
-                     (p `star` (ls2 `star` ctr)) }
-      (fp `star` frame) `star` (p `star` (ls2 `star` ctr));
-         (equiv) { star_associative (fp `star` frame) p (ls2 `star` ctr) }
-      (fp `star` frame `star` p) `star` (ls2 `star` ctr);
-         (equiv) { slprop_extensionality
-                     (fp `star` frame `star` p)
-                     (p `star` fp `star` frame)
-                  }
+// let with_inv_helper (fp frame ls1 ctr p ls2:slprop)
+//   : Lemma
+//       (requires ls1 `equiv` (p `star` ls2))
+//       (ensures
+//         (fp `star` frame `star` (ls1 `star` ctr)) `equiv`
+//         (p `star` fp `star` frame `star` (ls2 `star` ctr)))
+//   = calc (equiv) {
+//       ls1 `star` ctr;
+//          (equiv) { slprop_extensionality ls1 (p `star` ls2) }
+//       p `star` ls2 `star` ctr;
+//     };
+//     calc (equiv) {
+//       p `star` ls2 `star` ctr;
+//          (equiv) { star_associative p ls2 ctr }
+//       p `star` (ls2 `star` ctr);
+//     };
+//     calc (equiv) {
+//       fp `star` frame `star` p;
+//          (equiv) { star_commutative (fp `star` frame) p }
+//       p `star` (fp `star` frame);
+//          (equiv) { star_associative p fp frame }
+//       p `star` fp `star` frame;
+//     };
+//     calc (equiv) {
+//       fp `star` frame `star` (ls1 `star` ctr);
+//          (equiv) { equiv_ext_right (fp `star` frame)
+//                      (ls1 `star` ctr)
+//                      (p `star` ls2 `star` ctr) }
+//       (fp `star` frame) `star` (p `star` ls2 `star` ctr);
+//          (equiv) { equiv_ext_right (fp `star` frame)
+//                      (p `star` ls2 `star` ctr)
+//                      (p `star` (ls2 `star` ctr)) }
+//       (fp `star` frame) `star` (p `star` (ls2 `star` ctr));
+//          (equiv) { star_associative (fp `star` frame) p (ls2 `star` ctr) }
+//       (fp `star` frame `star` p) `star` (ls2 `star` ctr);
+//          (equiv) { slprop_extensionality
+//                      (fp `star` frame `star` p)
+//                      (p `star` fp `star` frame)
+//                   }
                   
-      (p `star` fp `star` frame) `star` (ls2 `star` ctr);
-    }
+//       (p `star` fp `star` frame) `star` (ls2 `star` ctr);
+//     }
 
-let token_of_inv #p (i:inv p) : (name_of_inv i >--> p) = let (| _, _, tok |) = i in tok
+// let token_of_inv #p (i:inv p) : (name_of_inv i >--> p) = let (| _, _, tok |) = i in tok
 
-let mst_aux #s rel a p q = x:s { p x } -> MST.mst #s rel a (fun s0 -> s0 == x) q
+// let mst_aux #s rel a p q = x:s { p x } -> MST.mst #s rel a (fun s0 -> s0 == x) q
 
-let with_invariant (#a:Type)
-                   (#fp:slprop)
-                   (#fp':a -> slprop)
-                   (#opened_invariants:inames)
-                   (#p:slprop)
-                   (i:inv p{not (mem_inv opened_invariants i)})
-                   (f:action_except a (add_inv opened_invariants i) (p `star` fp) (fun x -> p `star` fp' x))
-                   (frame:slprop)
-  : _MstTot a opened_invariants fp fp' frame
-  = let k1 (r:a)
-       : MST.mst_aux mem_evolves a
-          (fun m1 ->
-             inames_ok (set_add (name_of_inv i) opened_invariants) m1 /\
-             interp (p `star` fp' r `star` frame `star` locks_invariant (set_add (name_of_inv i) opened_invariants) m1) m1)
-          (fun _ x m1 ->
-             inames_ok opened_invariants m1 /\
-             interp (fp' x `star` frame `star` locks_invariant opened_invariants m1) m1)
-      = fun m1 ->
-          assert (interp (p `star` fp' r `star` frame `star` locks_invariant (set_add (name_of_inv i) opened_invariants) m1) m1);
-          assert (interp (p `star` fp' r `star` frame `star`
-          (lock_store_invariant (set_add (name_of_inv i) opened_invariants) m1.locks `star`
-            ctr_validity m1.ctr m1.ghost_ctr (heap_of_mem m1))) m1);
+// let with_invariant (#a:Type)
+//                    (#fp:slprop)
+//                    (#fp':a -> slprop)
+//                    (#opened_invariants:inames)
+//                    (#p:slprop)
+//                    (i:inv p{not (mem_inv opened_invariants i)})
+//                    (f:action_except a (add_inv opened_invariants i) (p `star` fp) (fun x -> p `star` fp' x))
+//                    (frame:slprop)
+//   : _MstTot a opened_invariants fp fp' frame
+//   = let k1 (r:a)
+//        : MST.mst_aux mem_evolves a
+//           (fun m1 ->
+//              inames_ok (set_add (name_of_inv i) opened_invariants) m1 /\
+//              interp (p `star` fp' r `star` frame `star` locks_invariant (set_add (name_of_inv i) opened_invariants) m1) m1)
+//           (fun _ x m1 ->
+//              inames_ok opened_invariants m1 /\
+//              interp (fp' x `star` frame `star` locks_invariant opened_invariants m1) m1)
+//       = fun m1 ->
+//           assert (interp (p `star` fp' r `star` frame `star` locks_invariant (set_add (name_of_inv i) opened_invariants) m1) m1);
+//           assert (interp (p `star` fp' r `star` frame `star`
+//           (lock_store_invariant (set_add (name_of_inv i) opened_invariants) m1.locks `star`
+//             ctr_validity m1.ctr m1.ghost_ctr (heap_of_mem m1))) m1);
 
-          let k2
-            : MST.mst_aux mem_evolves a
-                (fun m1 ->
-                  inames_ok (set_add (name_of_inv i) opened_invariants) m1 /\
-                  interp (p `star` fp' r `star` frame `star`
-                            (lock_store_invariant (set_add (name_of_inv i) opened_invariants) m1.locks `star`
-                              ctr_validity m1.ctr m1.ghost_ctr (heap_of_mem m1))) m1 /\
-                  iname_for_p_mem (name_of_inv i) p m1)
-                (fun _ x m1 ->
-                  inames_ok opened_invariants m1 /\
-                  interp (fp' x `star` frame `star` locks_invariant opened_invariants m1) m1)
-            = fun m1 ->
-                  move_invariant opened_invariants m1.locks p (name_of_inv i);
-                  assert (lock_store_invariant opened_invariants m1.locks `equiv`
-                      (p `star` lock_store_invariant (set_add (name_of_inv i) opened_invariants) m1.locks));
+//           let k2
+//             : MST.mst_aux mem_evolves a
+//                 (fun m1 ->
+//                   inames_ok (set_add (name_of_inv i) opened_invariants) m1 /\
+//                   interp (p `star` fp' r `star` frame `star`
+//                             (lock_store_invariant (set_add (name_of_inv i) opened_invariants) m1.locks `star`
+//                               ctr_validity m1.ctr m1.ghost_ctr (heap_of_mem m1))) m1 /\
+//                   iname_for_p_mem (name_of_inv i) p m1)
+//                 (fun _ x m1 ->
+//                   inames_ok opened_invariants m1 /\
+//                   interp (fp' x `star` frame `star` locks_invariant opened_invariants m1) m1)
+//             = fun m1 ->
+//                   move_invariant opened_invariants m1.locks p (name_of_inv i);
+//                   assert (lock_store_invariant opened_invariants m1.locks `equiv`
+//                       (p `star` lock_store_invariant (set_add (name_of_inv i) opened_invariants) m1.locks));
 
-                  with_inv_helper
-                    (fp' r)
-                    frame
-                    (lock_store_invariant opened_invariants m1.locks)
-                    (ctr_validity m1.ctr m1.ghost_ctr (heap_of_mem m1))
-                    p
-                    (lock_store_invariant (set_add (name_of_inv i) opened_invariants) m1.locks);
+//                   with_inv_helper
+//                     (fp' r)
+//                     frame
+//                     (lock_store_invariant opened_invariants m1.locks)
+//                     (ctr_validity m1.ctr m1.ghost_ctr (heap_of_mem m1))
+//                     p
+//                     (lock_store_invariant (set_add (name_of_inv i) opened_invariants) m1.locks);
 
-                  assert (interp (fp' r `star` frame `star` locks_invariant opened_invariants m1) m1);
+//                   assert (interp (fp' r `star` frame `star` locks_invariant opened_invariants m1) m1);
 
-                  assert (inames_ok opened_invariants m1);
-                  MST.weaken <| MST.return r
-          in
-          MST.weaken <|
-          MST.bind (MST.recall _ (token_of_inv i)) (fun _ -> MST.with_get k2)
-      in
-    let k0
-    : _mst_tot_aux a opened_invariants fp fp' frame
-          (iname_for_p_mem (name_of_inv i) p)
-    = fun m0 -> 
-        assert (iname_for_p (name_of_inv i) p m0.locks);
-        assert (interp (fp `star` frame `star` locks_invariant opened_invariants m0) m0);
-        assert (interp (fp `star` frame `star`
-          (lock_store_invariant opened_invariants m0.locks `star`
-          ctr_validity m0.ctr m0.ghost_ctr (heap_of_mem m0))) m0);
+//                   assert (inames_ok opened_invariants m1);
+//                   MST.weaken <| MST.return r
+//           in
+//           MST.weaken <|
+//           MST.bind (MST.recall _ (token_of_inv i)) (fun _ -> MST.with_get k2)
+//       in
+//     let k0
+//     : _mst_tot_aux a opened_invariants fp fp' frame
+//           (iname_for_p_mem (name_of_inv i) p)
+//     = fun m0 -> 
+//         assert (iname_for_p (name_of_inv i) p m0.locks);
+//         assert (interp (fp `star` frame `star` locks_invariant opened_invariants m0) m0);
+//         assert (interp (fp `star` frame `star`
+//           (lock_store_invariant opened_invariants m0.locks `star`
+//           ctr_validity m0.ctr m0.ghost_ctr (heap_of_mem m0))) m0);
 
-        move_invariant opened_invariants m0.locks p (name_of_inv i);
-        assert (lock_store_invariant opened_invariants m0.locks `equiv`
-                (p `star` lock_store_invariant (set_add (name_of_inv i) opened_invariants) m0.locks));
+//         move_invariant opened_invariants m0.locks p (name_of_inv i);
+//         assert (lock_store_invariant opened_invariants m0.locks `equiv`
+//                 (p `star` lock_store_invariant (set_add (name_of_inv i) opened_invariants) m0.locks));
 
-        with_inv_helper
-          fp
-          frame
-          (lock_store_invariant opened_invariants m0.locks)
-          (ctr_validity m0.ctr m0.ghost_ctr (heap_of_mem m0))
-          p
-          (lock_store_invariant (set_add (name_of_inv i) opened_invariants) m0.locks);
+//         with_inv_helper
+//           fp
+//           frame
+//           (lock_store_invariant opened_invariants m0.locks)
+//           (ctr_validity m0.ctr m0.ghost_ctr (heap_of_mem m0))
+//           p
+//           (lock_store_invariant (set_add (name_of_inv i) opened_invariants) m0.locks);
 
-        assert (interp (p `star` fp `star` frame `star` locks_invariant (set_add (name_of_inv i) opened_invariants) m0) m0);
-        MST.weaken <|
-        MST.bind (f frame) (fun r ->
-          MST.with_get (k1 r))
-    in
-    MST.weaken <|
-    MST.bind (MST.recall _ (token_of_inv i)) (fun _ ->
-    with_get_aux k0) 
+//         assert (interp (p `star` fp `star` frame `star` locks_invariant (set_add (name_of_inv i) opened_invariants) m0) m0);
+//         MST.weaken <|
+//         MST.bind (f frame) (fun r ->
+//           MST.with_get (k1 r))
+//     in
+//     MST.weaken <|
+//     MST.bind (MST.recall _ (token_of_inv i)) (fun _ ->
+//     with_get_aux k0) 
  
-let equiv_pqrs_p_qr_s (p q r s:slprop)
-  : Lemma ((p `star` q `star` r `star` s) `equiv`
-           (p `star` (q `star` r) `star` s))
-  = star_associative p q r;
-    slprop_extensionality
-      (p `star` q `star` r)
-      (p `star` (q `star` r))
+// let equiv_pqrs_p_qr_s (p q r s:slprop)
+//   : Lemma ((p `star` q `star` r `star` s) `equiv`
+//            (p `star` (q `star` r) `star` s))
+//   = star_associative p q r;
+//     slprop_extensionality
+//       (p `star` q `star` r)
+//       (p `star` (q `star` r))
 
-let frame (#a:Type)
-          (#opened_invariants:inames)
-          (#pre:slprop)
-          (#post:a -> slprop)
-          (frame:slprop)
-          ($f:action_except a opened_invariants pre post)
-          (frame0:slprop)
-  : _MstTot a opened_invariants (pre `star` frame) (fun x -> post x `star` frame) frame0
-  = let aux
-    : _mst_tot_aux a opened_invariants (pre `star` frame) (fun x -> post x `star` frame) frame0 (fun _ -> True)
-    = fun m0 ->
-        equiv_pqrs_p_qr_s pre frame frame0 (linv opened_invariants m0);
-        assert (interp (pre `star` frame `star` frame0 `star` linv opened_invariants m0) m0);
-        assert (interp (pre `star` (frame `star` frame0) `star` linv opened_invariants m0) m0);
-        MST.weaken <| 
-        MST.bind (f (frame `star` frame0)) (fun x ->
-          let k
-            : MST.mst_aux mem_evolves a 
-              (fun m1 ->
-                inames_ok opened_invariants m1 /\
-                interp (post x `star` (frame `star` frame0) `star` linv opened_invariants m1) m1)
-              (fun m0 x m1 -> 
-                inames_ok opened_invariants m1 /\
-                interp (post x `star` frame `star` frame0 `star` linv opened_invariants m1) m1)
-            = fun m1 -> 
-                equiv_pqrs_p_qr_s (post x) frame frame0 (linv opened_invariants m1);
-                assert (interp (post x `star` (frame `star` frame0) `star` linv opened_invariants m1) m1);
-                assert (interp (post x `star` frame `star` frame0 `star` linv opened_invariants m1) m1);
-                MST.weaken <| MST.return x
-          in
-          MST.with_get k
-        )
-    in
-    MST.weaken <| with_get_aux aux
+// let frame (#a:Type)
+//           (#opened_invariants:inames)
+//           (#pre:slprop)
+//           (#post:a -> slprop)
+//           (frame:slprop)
+//           ($f:action_except a opened_invariants pre post)
+//           (frame0:slprop)
+//   : _MstTot a opened_invariants (pre `star` frame) (fun x -> post x `star` frame) frame0
+//   = let aux
+//     : _mst_tot_aux a opened_invariants (pre `star` frame) (fun x -> post x `star` frame) frame0 (fun _ -> True)
+//     = fun m0 ->
+//         equiv_pqrs_p_qr_s pre frame frame0 (linv opened_invariants m0);
+//         assert (interp (pre `star` frame `star` frame0 `star` linv opened_invariants m0) m0);
+//         assert (interp (pre `star` (frame `star` frame0) `star` linv opened_invariants m0) m0);
+//         MST.weaken <| 
+//         MST.bind (f (frame `star` frame0)) (fun x ->
+//           let k
+//             : MST.mst_aux mem_evolves a 
+//               (fun m1 ->
+//                 inames_ok opened_invariants m1 /\
+//                 interp (post x `star` (frame `star` frame0) `star` linv opened_invariants m1) m1)
+//               (fun m0 x m1 -> 
+//                 inames_ok opened_invariants m1 /\
+//                 interp (post x `star` frame `star` frame0 `star` linv opened_invariants m1) m1)
+//             = fun m1 -> 
+//                 equiv_pqrs_p_qr_s (post x) frame frame0 (linv opened_invariants m1);
+//                 assert (interp (post x `star` (frame `star` frame0) `star` linv opened_invariants m1) m1);
+//                 assert (interp (post x `star` frame `star` frame0 `star` linv opened_invariants m1) m1);
+//                 MST.weaken <| MST.return x
+//           in
+//           MST.with_get k
+//         )
+//     in
+//     MST.weaken <| with_get_aux aux
 
-let pst_frame
-          (#a:Type)
-          (#mg:_)
-          (#opened_invariants:inames)
-          (#pre:slprop)
-          (#post:a -> slprop)
-          (frame:slprop)
-          ($f:_pst_action_except a mg opened_invariants pre post)
-: _pst_action_except a mg opened_invariants (pre `star` frame) (fun x -> post x `star` frame)
-= fun frame0 m0 ->
-    equiv_pqrs_p_qr_s pre frame frame0 (linv opened_invariants m0);
-    assert (interp (pre `star` frame `star` frame0 `star` linv opened_invariants m0) m0);
-    assert (interp (pre `star` (frame `star` frame0) `star` linv opened_invariants m0) m0);
-    let x, m1 = f (frame `star` frame0) m0 in
-    equiv_pqrs_p_qr_s (post x) frame frame0 (linv opened_invariants m1);
-    assert (interp (post x `star` (frame `star` frame0) `star` linv opened_invariants m1) m1);
-    assert (interp (post x `star` frame `star` frame0 `star` linv opened_invariants m1) m1);
-    x, m1
+// let pst_frame
+//           (#a:Type)
+//           (#mg:_)
+//           (#opened_invariants:inames)
+//           (#pre:slprop)
+//           (#post:a -> slprop)
+//           (frame:slprop)
+//           ($f:_pst_action_except a mg opened_invariants pre post)
+// : _pst_action_except a mg opened_invariants (pre `star` frame) (fun x -> post x `star` frame)
+// = fun frame0 m0 ->
+//     equiv_pqrs_p_qr_s pre frame frame0 (linv opened_invariants m0);
+//     assert (interp (pre `star` frame `star` frame0 `star` linv opened_invariants m0) m0);
+//     assert (interp (pre `star` (frame `star` frame0) `star` linv opened_invariants m0) m0);
+//     let x, m1 = f (frame `star` frame0) m0 in
+//     equiv_pqrs_p_qr_s (post x) frame frame0 (linv opened_invariants m1);
+//     assert (interp (post x `star` (frame `star` frame0) `star` linv opened_invariants m1) m1);
+//     assert (interp (post x `star` frame `star` frame0 `star` linv opened_invariants m1) m1);
+//     x, m1
 
-let change_slprop (#opened_invariants:inames)
-                  (p q:slprop)
-                  (proof: (m:mem -> Lemma (requires interp p m) (ensures interp q m)))
-: pst_ghost_action_except unit opened_invariants p (fun _ -> q)
-= let proof (h:H.heap)
-    : Lemma (requires H.interp p h)
-            (ensures H.interp q h)
-    = proof (mem_of_heap h)
-  in
-  lift_tot_action (lift_heap_action opened_invariants (H.change_slprop p q proof))
+// let change_slprop (#opened_invariants:inames)
+//                   (p q:slprop)
+//                   (proof: (m:mem -> Lemma (requires interp p m) (ensures interp q m)))
+// : pst_ghost_action_except unit opened_invariants p (fun _ -> q)
+// = let proof (h:H.heap)
+//     : Lemma (requires H.interp p h)
+//             (ensures H.interp q h)
+//     = proof (mem_of_heap h)
+//   in
+//   lift_tot_action (lift_heap_action opened_invariants (H.change_slprop p q proof))
 
-let witness_h_exists #opened_invariants #a p =
-  lift_tot_action_with_frame (lift_heap_action_with_frame opened_invariants (H.elim_exists p))
+// let witness_h_exists #opened_invariants #a p =
+//   lift_tot_action_with_frame (lift_heap_action_with_frame opened_invariants (H.elim_exists p))
 
-let intro_exists #opened_invariants #a p x = 
-  lift_tot_action_with_frame (lift_heap_action_with_frame opened_invariants (H.intro_exists p x))
+// let intro_exists #opened_invariants #a p x = 
+//   lift_tot_action_with_frame (lift_heap_action_with_frame opened_invariants (H.intro_exists p x))
 
-let lift_h_exists #opened_invariants p = lift_tot_action (lift_heap_action opened_invariants (H.lift_exists p))
+// let lift_h_exists #opened_invariants p = lift_tot_action (lift_heap_action opened_invariants (H.lift_exists p))
 
-let elim_pure #opened_invariants p = lift_tot_action (lift_heap_action opened_invariants (H.elim_pure p))
+// let elim_pure #opened_invariants p = lift_tot_action (lift_heap_action opened_invariants (H.elim_pure p))
 
-let intro_pure #opened_invariants p pf = lift_tot_action (lift_heap_action opened_invariants (H.intro_pure p pf))
+// let intro_pure #opened_invariants p pf = lift_tot_action (lift_heap_action opened_invariants (H.intro_pure p pf))
 
-let drop #o p = lift_tot_action (lift_heap_action o (H.drop p))
+// let drop #o p = lift_tot_action (lift_heap_action o (H.drop p))
 
-let lift_ghost
-      (#a:Type)
-      #opened_invariants #p #q
-      (ni_a:non_info a)
-      (f:erased (pst_ghost_action_except a opened_invariants p q))
-  : pst_ghost_action_except a opened_invariants p q
-  = fun frame m0 ->
-      let xm1 : erased (a * full_mem) = 
-        let ff = reveal f in
-        let x, m1 = ff frame m0 in
-        assert (maybe_ghost_action true m0 m1);
-        hide (x, m1)
-      in
-      let m1' : erased full_mem = hide (snd (reveal xm1)) in
-      let x' : erased a = hide (fst (reveal xm1)) in
-      let m1 : full_mem = 
-        { m0 with heap = H.upd_ghost_heap m0.heap (hide (m1'.heap));
-                  ghost_ctr = (reveal m1').ghost_ctr } in
-      let x = ni_a (hide (fst (reveal xm1))) in
-      (x, m1)
+// let lift_ghost
+//       (#a:Type)
+//       #opened_invariants #p #q
+//       (ni_a:non_info a)
+//       (f:erased (pst_ghost_action_except a opened_invariants p q))
+//   : pst_ghost_action_except a opened_invariants p q
+//   = fun frame m0 ->
+//       let xm1 : erased (a * full_mem) = 
+//         let ff = reveal f in
+//         let x, m1 = ff frame m0 in
+//         assert (maybe_ghost_action true m0 m1);
+//         hide (x, m1)
+//       in
+//       let m1' : erased full_mem = hide (snd (reveal xm1)) in
+//       let x' : erased a = hide (fst (reveal xm1)) in
+//       let m1 : full_mem = 
+//         { m0 with heap = H.upd_ghost_heap m0.heap (hide (m1'.heap));
+//                   ghost_ctr = (reveal m1').ghost_ctr } in
+//       let x = ni_a (hide (fst (reveal xm1))) in
+//       (x, m1)
 
-(* Concrete small refs *)
-let pts_to = H.pts_to
+// (* Concrete small refs *)
+// let pts_to = H.pts_to
 
-let sel_action #a #pcm e r v0
-  = lift_tot_action (lift_heap_action e (H.sel_action #a #pcm r v0))
+// let sel_action #a #pcm e r v0
+//   = lift_tot_action (lift_heap_action e (H.sel_action #a #pcm r v0))
 
-let upd_action #a #pcm e r v0 v1
-  = lift_tot_action (lift_heap_action e (H.upd_action #a #pcm r v0 v1))
+// let upd_action #a #pcm e r v0 v1
+//   = lift_tot_action (lift_heap_action e (H.upd_action #a #pcm r v0 v1))
 
-let free_action #a #pcm e r v0
-  = lift_tot_action (lift_heap_action e (H.free_action #a #pcm r v0))
+// let free_action #a #pcm e r v0
+//   = lift_tot_action (lift_heap_action e (H.free_action #a #pcm r v0))
 
-let split_action #a #pcm e r v0 v1
-  = lift_tot_action (lift_heap_action e (H.split_action #a #pcm r v0 v1))
+// let split_action #a #pcm e r v0 v1
+//   = lift_tot_action (lift_heap_action e (H.split_action #a #pcm r v0 v1))
 
-let gather_action #a #pcm e r v0 v1
-  = lift_tot_action (lift_heap_action e (H.gather_action #a #pcm r v0 v1))
+// let gather_action #a #pcm e r v0 v1
+//   = lift_tot_action (lift_heap_action e (H.gather_action #a #pcm r v0 v1))
 
-let weaken (p q r:slprop) (h:H.hheap (p `star` q) { H.stronger q r })
-  : H.hheap (p `star` r)
-  = H.weaken p q r h; h
+// let weaken (p q r:slprop) (h:H.hheap (p `star` q) { H.stronger q r })
+//   : H.hheap (p `star` r)
+//   = H.weaken p q r h; h
 
-let weaken_pure (q r: prop)
-  : Lemma
-    (requires (q ==> r))
-    (ensures H.stronger (H.pure q) (H.pure r))
-  = let aux (h:H.heap)
-        : Lemma (ensures (H.interp (H.pure q) h ==> H.interp (H.pure r) h))
-                [SMTPat ()]
-        = H.pure_interp q h;
-          H.pure_interp r h
-    in
-    ()
+// let weaken_pure (q r: prop)
+//   : Lemma
+//     (requires (q ==> r))
+//     (ensures H.stronger (H.pure q) (H.pure r))
+//   = let aux (h:H.heap)
+//         : Lemma (ensures (H.interp (H.pure q) h ==> H.interp (H.pure r) h))
+//                 [SMTPat ()]
+//         = H.pure_interp q h;
+//           H.pure_interp r h
+//     in
+//     ()
 
-let inc_ctr (#p:slprop) #e (m:hmem_with_inv_except e p)
-  : m':hmem_with_inv_except e p{m'.ctr = m.ctr + 1 /\ H.stronger (linv e m) (linv e m')}
-  = let m' : mem = { m with ctr = m.ctr + 1} in
-    assert (interp (p `star` linv e m) m');
-    assert (linv e m == lock_store_invariant e m.locks
-                        `star`
-                        ctr_validity m.ctr m.ghost_ctr (heap_of_mem m));
-    assert (linv e m' == lock_store_invariant e m.locks
-                         `star`
-                        ctr_validity (m.ctr + 1) m.ghost_ctr (heap_of_mem m));
-    H.weaken_free_above CONCRETE (heap_of_mem m) m.ctr (m.ctr + 1);
-    weaken_pure (heap_ctr_valid m.ctr m.ghost_ctr (heap_of_mem m))
-                (heap_ctr_valid (m.ctr + 1) m.ghost_ctr (heap_of_mem m));
-    assert (H.stronger
-                  (ctr_validity m.ctr m.ghost_ctr (heap_of_mem m))
-                  (ctr_validity (m.ctr + 1) m.ghost_ctr (heap_of_mem m)));
-    H.star_associative p (lock_store_invariant e m.locks)
-                         (ctr_validity m.ctr m.ghost_ctr (heap_of_mem m));
-    H.stronger_star (lock_store_invariant e m.locks)
-                    (ctr_validity m.ctr m.ghost_ctr (heap_of_mem m))
-                    (ctr_validity (m.ctr + 1) m.ghost_ctr (heap_of_mem m));
-    H.weaken (p `star` lock_store_invariant e m.locks)
-             (ctr_validity m.ctr m.ghost_ctr (heap_of_mem m))
-             (ctr_validity (m.ctr + 1) m.ghost_ctr (heap_of_mem m))
-             (heap_of_mem m');
-    H.star_associative p (lock_store_invariant e m.locks)
-                         (ctr_validity (m.ctr + 1) m.ghost_ctr (heap_of_mem m));
-    let m' : hmem_with_inv_except e p = m' in
-    m'
+// let inc_ctr (#p:slprop) #e (m:hmem_with_inv_except e p)
+//   : m':hmem_with_inv_except e p{m'.ctr = m.ctr + 1 /\ H.stronger (linv e m) (linv e m')}
+//   = let m' : mem = { m with ctr = m.ctr + 1} in
+//     assert (interp (p `star` linv e m) m');
+//     assert (linv e m == lock_store_invariant e m.locks
+//                         `star`
+//                         ctr_validity m.ctr m.ghost_ctr (heap_of_mem m));
+//     assert (linv e m' == lock_store_invariant e m.locks
+//                          `star`
+//                         ctr_validity (m.ctr + 1) m.ghost_ctr (heap_of_mem m));
+//     H.weaken_free_above CONCRETE (heap_of_mem m) m.ctr (m.ctr + 1);
+//     weaken_pure (heap_ctr_valid m.ctr m.ghost_ctr (heap_of_mem m))
+//                 (heap_ctr_valid (m.ctr + 1) m.ghost_ctr (heap_of_mem m));
+//     assert (H.stronger
+//                   (ctr_validity m.ctr m.ghost_ctr (heap_of_mem m))
+//                   (ctr_validity (m.ctr + 1) m.ghost_ctr (heap_of_mem m)));
+//     H.star_associative p (lock_store_invariant e m.locks)
+//                          (ctr_validity m.ctr m.ghost_ctr (heap_of_mem m));
+//     H.stronger_star (lock_store_invariant e m.locks)
+//                     (ctr_validity m.ctr m.ghost_ctr (heap_of_mem m))
+//                     (ctr_validity (m.ctr + 1) m.ghost_ctr (heap_of_mem m));
+//     H.weaken (p `star` lock_store_invariant e m.locks)
+//              (ctr_validity m.ctr m.ghost_ctr (heap_of_mem m))
+//              (ctr_validity (m.ctr + 1) m.ghost_ctr (heap_of_mem m))
+//              (heap_of_mem m');
+//     H.star_associative p (lock_store_invariant e m.locks)
+//                          (ctr_validity (m.ctr + 1) m.ghost_ctr (heap_of_mem m));
+//     let m' : hmem_with_inv_except e p = m' in
+//     m'
 
-let with_fresh_counter (#t:Type u#a) (#post:t -> slprop u#m) (e:inames)
-  (f: (addr:nat ->
-        H.action #MUTABLE #(Some CONCRETE)
-          #(fun h -> h `H.free_above_addr CONCRETE` addr)
-          #(fun h -> h `H.free_above_addr CONCRETE` (addr + 1))      
-          emp 
-          t
-          post))
-: pst_action_except t e emp post
-= let f : refined_pre_action false e emp t post
-    = fun m0 ->
-        let h = hheap_of_hmem m0 in
-        let (|r, h'|) = f m0.ctr h in
-        let m' : hmem_with_inv_except e emp = inc_ctr m0 in
-        let h' : H.hheap (post r `star` linv e m') = weaken _ (linv e m0) (linv e m') h' in
-        let m1 : hmem_with_inv_except e (post r) = hmem_of_hheap m' h' in
-        let aux (frame:slprop)
-          : Lemma
-            (requires
-               interp ((emp `star` frame) `star` linv e m0) m0)
-            (ensures
-               interp ((post r `star` frame) `star` linv e m1) m1 /\
-               mem_evolves m0 m1)
-            [SMTPat (emp `star` frame)]
-          = star_associative emp frame (linv e m0);
-            assert (H.interp (emp `star` (frame `star` linv e m0)) h);
-            assert (H.interp (post r `star` (frame `star` linv e m0)) h');
-            star_associative (post r) frame (linv e m0);
-            assert (H.interp ((post r `star` frame) `star` linv e m0) h');
-            assert (H.stronger (linv e m0) (linv e m'));
-            assert (H.equiv (linv e m') (linv e m1));
-            assert (H.stronger (linv e m0) (linv e m1));
-            let h' : H.hheap ((post r `star` frame) `star` linv e m1) = weaken _ (linv e m0) (linv e m1) h' in
-            assert (H.interp ((post r `star` frame) `star` linv e m1) h')
-        in
-        assert (frame_related_mems emp (post r) e m0 m1);
-        (| r, m1 |)
-    in
-    lift_tot_action (refined_pre_action_as_action f)
-
-
-let alloc_action #a #pcm e x
-  = with_fresh_counter e (H.extend #a #pcm x)
-
-let select_refine #a #p e r x f
-  = lift_tot_action (lift_heap_action e (H.select_refine #a #p r x f))
-
-let upd_gen #a #p e r x y f
-  = lift_tot_action (lift_heap_action e (H.upd_gen_action r x y f))
-
-let pts_to_not_null_action
-      (#a:Type u#a) (#pcm:pcm a)
-      (e:inames)
-      (r:erased (ref a pcm))
-      (v:Ghost.erased a)
-: pst_ghost_action_except (squash (not (is_null r))) e
-    (pts_to r v)
-    (fun _ -> pts_to r v)
-= lift_tot_action (lift_heap_action e (H.pts_to_not_null_action #a #pcm r v))
-
-let ghost_ref = H.ghost_ref
-let ghost_pts_to = H.ghost_pts_to
+// let with_fresh_counter (#t:Type u#a) (#post:t -> slprop u#m) (e:inames)
+//   (f: (addr:nat ->
+//         H.action #MUTABLE #(Some CONCRETE)
+//           #(fun h -> h `H.free_above_addr CONCRETE` addr)
+//           #(fun h -> h `H.free_above_addr CONCRETE` (addr + 1))      
+//           emp 
+//           t
+//           post))
+// : pst_action_except t e emp post
+// = let f : refined_pre_action false e emp t post
+//     = fun m0 ->
+//         let h = hheap_of_hmem m0 in
+//         let (|r, h'|) = f m0.ctr h in
+//         let m' : hmem_with_inv_except e emp = inc_ctr m0 in
+//         let h' : H.hheap (post r `star` linv e m') = weaken _ (linv e m0) (linv e m') h' in
+//         let m1 : hmem_with_inv_except e (post r) = hmem_of_hheap m' h' in
+//         let aux (frame:slprop)
+//           : Lemma
+//             (requires
+//                interp ((emp `star` frame) `star` linv e m0) m0)
+//             (ensures
+//                interp ((post r `star` frame) `star` linv e m1) m1 /\
+//                mem_evolves m0 m1)
+//             [SMTPat (emp `star` frame)]
+//           = star_associative emp frame (linv e m0);
+//             assert (H.interp (emp `star` (frame `star` linv e m0)) h);
+//             assert (H.interp (post r `star` (frame `star` linv e m0)) h');
+//             star_associative (post r) frame (linv e m0);
+//             assert (H.interp ((post r `star` frame) `star` linv e m0) h');
+//             assert (H.stronger (linv e m0) (linv e m'));
+//             assert (H.equiv (linv e m') (linv e m1));
+//             assert (H.stronger (linv e m0) (linv e m1));
+//             let h' : H.hheap ((post r `star` frame) `star` linv e m1) = weaken _ (linv e m0) (linv e m1) h' in
+//             assert (H.interp ((post r `star` frame) `star` linv e m1) h')
+//         in
+//         assert (frame_related_mems emp (post r) e m0 m1);
+//         (| r, m1 |)
+//     in
+//     lift_tot_action (refined_pre_action_as_action f)
 
 
-let inc_ghost_ctr (#p:slprop) #e (m:hmem_with_inv_except e p)
-  : m':hmem_with_inv_except e p{reveal m'.ghost_ctr = m.ghost_ctr + 1 /\ H.stronger (linv e m) (linv e m')}
-  = let m' : mem = { m with ghost_ctr = m.ghost_ctr + 1} in
-    assert (interp (p `star` linv e m) m');
-    assert (linv e m == lock_store_invariant e m.locks
-                        `star`
-                        ctr_validity m.ctr m.ghost_ctr (heap_of_mem m));
-    assert (linv e m' == lock_store_invariant e m.locks
-                         `star`
-                        ctr_validity m.ctr (m.ghost_ctr + 1) (heap_of_mem m));
-    H.weaken_free_above GHOST (heap_of_mem m) m.ghost_ctr (m.ghost_ctr + 1);
-    weaken_pure (heap_ctr_valid m.ctr m.ghost_ctr (heap_of_mem m))
-                (heap_ctr_valid m.ctr (m.ghost_ctr + 1) (heap_of_mem m));
-    assert (H.stronger
-                  (ctr_validity m.ctr m.ghost_ctr (heap_of_mem m))
-                  (ctr_validity m.ctr (m.ghost_ctr + 1) (heap_of_mem m)));
-    H.star_associative p (lock_store_invariant e m.locks)
-                         (ctr_validity m.ctr m.ghost_ctr (heap_of_mem m));
-    H.stronger_star (lock_store_invariant e m.locks)
-                    (ctr_validity m.ctr m.ghost_ctr (heap_of_mem m))
-                    (ctr_validity m.ctr (m.ghost_ctr + 1) (heap_of_mem m));
-    H.weaken (p `star` lock_store_invariant e m.locks)
-             (ctr_validity m.ctr m.ghost_ctr (heap_of_mem m))
-             (ctr_validity m.ctr (m.ghost_ctr + 1) (heap_of_mem m))
-             (heap_of_mem m');
-    H.star_associative p (lock_store_invariant e m.locks)
-                         (ctr_validity m.ctr (m.ghost_ctr + 1) (heap_of_mem m));
-    let m' : hmem_with_inv_except e p = m' in
-    m'
+// let alloc_action #a #pcm e x
+//   = with_fresh_counter e (H.extend #a #pcm x)
 
-let with_fresh_ghost_counter (#t:Type u#a) (#post:t -> slprop u#m) (e:inames)
-  (f: (addr:erased nat ->
-        H.action #ONLY_GHOST #(Some GHOST)
-          #(fun h -> h `H.free_above_addr GHOST` addr)
-          #(fun h -> h `H.free_above_addr GHOST` (addr + 1))      
-          emp 
-          t
-          post))
-: pst_ghost_action_except t e emp post
-  = let f : refined_pre_action true e emp t post
-    = fun m0 ->
-        let h = hheap_of_hmem m0 in
-        let (|r, h'|) = f m0.ghost_ctr h in
-        let m' : hmem_with_inv_except e emp = inc_ghost_ctr m0 in
-        let h' : H.hheap (post r `star` linv e m') = weaken _ (linv e m0) (linv e m') h' in
-        let m1 : hmem_with_inv_except e (post r) = hmem_of_hheap m' h' in
-        let aux (frame:slprop)
-          : Lemma
-            (requires
-               interp ((emp `star` frame) `star` linv e m0) m0)
-            (ensures
-               interp ((post r `star` frame) `star` linv e m1) m1 /\
-               mem_evolves m0 m1)
-            [SMTPat (emp `star` frame)]
-          = star_associative emp frame (linv e m0);
-            assert (H.interp (emp `star` (frame `star` linv e m0)) h);
-            assert (H.interp (post r `star` (frame `star` linv e m0)) h');
-            star_associative (post r) frame (linv e m0);
-            assert (H.interp ((post r `star` frame) `star` linv e m0) h');
-            assert (H.stronger (linv e m0) (linv e m'));
-            assert (H.equiv (linv e m') (linv e m1));
-            assert (H.stronger (linv e m0) (linv e m1));
-            let h' : H.hheap ((post r `star` frame) `star` linv e m1) = weaken _ (linv e m0) (linv e m1) h' in
-            assert (H.interp ((post r `star` frame) `star` linv e m1) h')
-        in
-        assert (frame_related_mems emp (post r) e m0 m1);
-        (| r, m1 |)
-    in
-    lift_tot_action (refined_pre_action_as_action f)
+// let select_refine #a #p e r x f
+//   = lift_tot_action (lift_heap_action e (H.select_refine #a #p r x f))
 
-let ghost_alloc #e #a #pcm x
-  = with_fresh_ghost_counter e (H.ghost_extend #a #pcm x)
+// let upd_gen #a #p e r x y f
+//   = lift_tot_action (lift_heap_action e (H.upd_gen_action r x y f))
 
-let ghost_read #o #a #p r x f
-  = lift_tot_action (lift_heap_action o (H.ghost_read #a #p r x f))
-let ghost_write #o #a #p r x y f
-  = lift_tot_action (lift_heap_action o (H.ghost_write #a #p r x y f)) 
-let ghost_share #o #a #p r v0 v1
-  = lift_tot_action (lift_heap_action o (H.ghost_share #a #p r v0 v1))
-let ghost_gather #o #a #p r v0 v1
-  = lift_tot_action (lift_heap_action o (H.ghost_gather #a #p r v0 v1))
+// let pts_to_not_null_action
+//       (#a:Type u#a) (#pcm:pcm a)
+//       (e:inames)
+//       (r:erased (ref a pcm))
+//       (v:Ghost.erased a)
+// : pst_ghost_action_except (squash (not (is_null r))) e
+//     (pts_to r v)
+//     (fun _ -> pts_to r v)
+// = lift_tot_action (lift_heap_action e (H.pts_to_not_null_action #a #pcm r v))
 
-let big_pts_to = H.big_pts_to
-
-let big_sel_action #a #pcm e r v0
-  = lift_tot_action (lift_heap_action e (H.big_sel_action #a #pcm r v0))
-
-let big_upd_action #a #pcm e r v0 v1
-  = lift_tot_action (lift_heap_action e (H.big_upd_action #a #pcm r v0 v1))
-
-let big_free_action #a #pcm e r v0
-  = lift_tot_action (lift_heap_action e (H.big_free_action #a #pcm r v0))
-
-let big_split_action #a #pcm e r v0 v1
-  = lift_tot_action (lift_heap_action e (H.big_split_action #a #pcm r v0 v1))
-
-let big_gather_action #a #pcm e r v0 v1
-  = lift_tot_action (lift_heap_action e (H.big_gather_action #a #pcm r v0 v1))
+// let ghost_ref = H.ghost_ref
+// let ghost_pts_to = H.ghost_pts_to
 
 
-let big_alloc_action #a #pcm e x
-  = with_fresh_counter e (H.big_extend #a #pcm x)
+// let inc_ghost_ctr (#p:slprop) #e (m:hmem_with_inv_except e p)
+//   : m':hmem_with_inv_except e p{reveal m'.ghost_ctr = m.ghost_ctr + 1 /\ H.stronger (linv e m) (linv e m')}
+//   = let m' : mem = { m with ghost_ctr = m.ghost_ctr + 1} in
+//     assert (interp (p `star` linv e m) m');
+//     assert (linv e m == lock_store_invariant e m.locks
+//                         `star`
+//                         ctr_validity m.ctr m.ghost_ctr (heap_of_mem m));
+//     assert (linv e m' == lock_store_invariant e m.locks
+//                          `star`
+//                         ctr_validity m.ctr (m.ghost_ctr + 1) (heap_of_mem m));
+//     H.weaken_free_above GHOST (heap_of_mem m) m.ghost_ctr (m.ghost_ctr + 1);
+//     weaken_pure (heap_ctr_valid m.ctr m.ghost_ctr (heap_of_mem m))
+//                 (heap_ctr_valid m.ctr (m.ghost_ctr + 1) (heap_of_mem m));
+//     assert (H.stronger
+//                   (ctr_validity m.ctr m.ghost_ctr (heap_of_mem m))
+//                   (ctr_validity m.ctr (m.ghost_ctr + 1) (heap_of_mem m)));
+//     H.star_associative p (lock_store_invariant e m.locks)
+//                          (ctr_validity m.ctr m.ghost_ctr (heap_of_mem m));
+//     H.stronger_star (lock_store_invariant e m.locks)
+//                     (ctr_validity m.ctr m.ghost_ctr (heap_of_mem m))
+//                     (ctr_validity m.ctr (m.ghost_ctr + 1) (heap_of_mem m));
+//     H.weaken (p `star` lock_store_invariant e m.locks)
+//              (ctr_validity m.ctr m.ghost_ctr (heap_of_mem m))
+//              (ctr_validity m.ctr (m.ghost_ctr + 1) (heap_of_mem m))
+//              (heap_of_mem m');
+//     H.star_associative p (lock_store_invariant e m.locks)
+//                          (ctr_validity m.ctr (m.ghost_ctr + 1) (heap_of_mem m));
+//     let m' : hmem_with_inv_except e p = m' in
+//     m'
 
-let big_select_refine #a #p e r x f
-  = lift_tot_action (lift_heap_action e (H.big_select_refine #a #p r x f))
+// let with_fresh_ghost_counter (#t:Type u#a) (#post:t -> slprop u#m) (e:inames)
+//   (f: (addr:erased nat ->
+//         H.action #ONLY_GHOST #(Some GHOST)
+//           #(fun h -> h `H.free_above_addr GHOST` addr)
+//           #(fun h -> h `H.free_above_addr GHOST` (addr + 1))      
+//           emp 
+//           t
+//           post))
+// : pst_ghost_action_except t e emp post
+//   = let f : refined_pre_action true e emp t post
+//     = fun m0 ->
+//         let h = hheap_of_hmem m0 in
+//         let (|r, h'|) = f m0.ghost_ctr h in
+//         let m' : hmem_with_inv_except e emp = inc_ghost_ctr m0 in
+//         let h' : H.hheap (post r `star` linv e m') = weaken _ (linv e m0) (linv e m') h' in
+//         let m1 : hmem_with_inv_except e (post r) = hmem_of_hheap m' h' in
+//         let aux (frame:slprop)
+//           : Lemma
+//             (requires
+//                interp ((emp `star` frame) `star` linv e m0) m0)
+//             (ensures
+//                interp ((post r `star` frame) `star` linv e m1) m1 /\
+//                mem_evolves m0 m1)
+//             [SMTPat (emp `star` frame)]
+//           = star_associative emp frame (linv e m0);
+//             assert (H.interp (emp `star` (frame `star` linv e m0)) h);
+//             assert (H.interp (post r `star` (frame `star` linv e m0)) h');
+//             star_associative (post r) frame (linv e m0);
+//             assert (H.interp ((post r `star` frame) `star` linv e m0) h');
+//             assert (H.stronger (linv e m0) (linv e m'));
+//             assert (H.equiv (linv e m') (linv e m1));
+//             assert (H.stronger (linv e m0) (linv e m1));
+//             let h' : H.hheap ((post r `star` frame) `star` linv e m1) = weaken _ (linv e m0) (linv e m1) h' in
+//             assert (H.interp ((post r `star` frame) `star` linv e m1) h')
+//         in
+//         assert (frame_related_mems emp (post r) e m0 m1);
+//         (| r, m1 |)
+//     in
+//     lift_tot_action (refined_pre_action_as_action f)
 
-let big_upd_gen #a #p e r x y f
-  = lift_tot_action (lift_heap_action e (H.big_upd_gen_action r x y f))
+// let ghost_alloc #e #a #pcm x
+//   = with_fresh_ghost_counter e (H.ghost_extend #a #pcm x)
 
-let big_pts_to_not_null_action
-      (#a:Type u#(ua + 1)) (#pcm:pcm a)
-      (e:inames)
-      (r:erased (ref a pcm))
-      (v:Ghost.erased a)
-: pst_ghost_action_except (squash (not (is_null r))) e
-    (big_pts_to r v)
-    (fun _ -> big_pts_to r v)
-= lift_tot_action (lift_heap_action e (H.big_pts_to_not_null_action #a #pcm r v))
+// let ghost_read #o #a #p r x f
+//   = lift_tot_action (lift_heap_action o (H.ghost_read #a #p r x f))
+// let ghost_write #o #a #p r x y f
+//   = lift_tot_action (lift_heap_action o (H.ghost_write #a #p r x y f)) 
+// let ghost_share #o #a #p r v0 v1
+//   = lift_tot_action (lift_heap_action o (H.ghost_share #a #p r v0 v1))
+// let ghost_gather #o #a #p r v0 v1
+//   = lift_tot_action (lift_heap_action o (H.ghost_gather #a #p r v0 v1))
+
+// let big_pts_to = H.big_pts_to
+
+// let big_sel_action #a #pcm e r v0
+//   = lift_tot_action (lift_heap_action e (H.big_sel_action #a #pcm r v0))
+
+// let big_upd_action #a #pcm e r v0 v1
+//   = lift_tot_action (lift_heap_action e (H.big_upd_action #a #pcm r v0 v1))
+
+// let big_free_action #a #pcm e r v0
+//   = lift_tot_action (lift_heap_action e (H.big_free_action #a #pcm r v0))
+
+// let big_split_action #a #pcm e r v0 v1
+//   = lift_tot_action (lift_heap_action e (H.big_split_action #a #pcm r v0 v1))
+
+// let big_gather_action #a #pcm e r v0 v1
+//   = lift_tot_action (lift_heap_action e (H.big_gather_action #a #pcm r v0 v1))
 
 
-let big_ghost_pts_to = H.big_ghost_pts_to
-let big_ghost_alloc #e #a #pcm x
-  = with_fresh_ghost_counter e (H.big_ghost_extend #a #pcm x)
-let big_ghost_read #o #a #p r x f
-  = lift_tot_action (lift_heap_action o (H.big_ghost_read #a #p r x f))
-let big_ghost_write #o #a #p r x y f
-  = lift_tot_action (lift_heap_action o (H.big_ghost_write #a #p r x y f)) 
-let big_ghost_share #o #a #p r v0 v1
-  = lift_tot_action (lift_heap_action o (H.big_ghost_share #a #p r v0 v1))
-let big_ghost_gather #o #a #p r v0 v1
-  = lift_tot_action (lift_heap_action o (H.big_ghost_gather #a #p r v0 v1))
+// let big_alloc_action #a #pcm e x
+//   = with_fresh_counter e (H.big_extend #a #pcm x)
+
+// let big_select_refine #a #p e r x f
+//   = lift_tot_action (lift_heap_action e (H.big_select_refine #a #p r x f))
+
+// let big_upd_gen #a #p e r x y f
+//   = lift_tot_action (lift_heap_action e (H.big_upd_gen_action r x y f))
+
+// let big_pts_to_not_null_action
+//       (#a:Type u#(ua + 1)) (#pcm:pcm a)
+//       (e:inames)
+//       (r:erased (ref a pcm))
+//       (v:Ghost.erased a)
+// : pst_ghost_action_except (squash (not (is_null r))) e
+//     (big_pts_to r v)
+//     (fun _ -> big_pts_to r v)
+// = lift_tot_action (lift_heap_action e (H.big_pts_to_not_null_action #a #pcm r v))
+
+
+// let big_ghost_pts_to = H.big_ghost_pts_to
+// let big_ghost_alloc #e #a #pcm x
+//   = with_fresh_ghost_counter e (H.big_ghost_extend #a #pcm x)
+// let big_ghost_read #o #a #p r x f
+//   = lift_tot_action (lift_heap_action o (H.big_ghost_read #a #p r x f))
+// let big_ghost_write #o #a #p r x y f
+//   = lift_tot_action (lift_heap_action o (H.big_ghost_write #a #p r x y f)) 
+// let big_ghost_share #o #a #p r v0 v1
+//   = lift_tot_action (lift_heap_action o (H.big_ghost_share #a #p r v0 v1))
+// let big_ghost_gather #o #a #p r v0 v1
+//   = lift_tot_action (lift_heap_action o (H.big_ghost_gather #a #p r v0 v1))
 
